new/proof/sync/atomic.v
@@ -34,6 +34,37 @@ Proof.
   wp_auto. iFrame "∗#". done.
 Qed.
 
+Lemma noCopy_emp l dq :
+  ⊢ l ↦{dq} atomic.noCopy.mk.
+Proof.
+  rewrite typed_pointsto_unseal /typed_pointsto_def /=.
+  replace (flatten_struct (# _)) with ([] : list val).
+  - auto.
+  - rewrite to_val_unseal /=.
+    rewrite struct.val_aux_nil to_val_unseal //.
+Qed.
+
+Lemma align_emp l dq :
+  ⊢ l ↦{dq} atomic.align64.mk.
+Proof.
+  rewrite typed_pointsto_unseal /typed_pointsto_def /=.
+  replace (flatten_struct (#_)) with ([] : list val).
+  - auto.
+  - rewrite to_val_unseal /=.
+    rewrite struct.val_aux_nil to_val_unseal //.
+Qed.
+
+(* 64-bit structs have an extra field (align64) *)
+Definition own_Uint64 (u : loc) dq (v : w64) : iProp Σ :=
+  u ↦{dq} atomic.Uint64.mk (default_val _) (default_val _) v.
+Definition own_Int64 (u : loc) dq (v : w64) : iProp Σ :=
+  u ↦{dq} atomic.Int64.mk (default_val _) (default_val _) v.
+Definition own_Uint32 (u : loc) dq (v : w32) : iProp Σ :=
+  u ↦{dq} atomic.Uint32.mk (default_val _) v.
+Definition own_Int32 (u : loc) dq (v : w32) : iProp Σ :=
+  u ↦{dq} atomic.Int32.mk (default_val _) v.
+
+(* BEGIN TEMPLATE *)
 Lemma wp_LoadUint64 (addr : loc) dq :
   ∀ Φ,
   is_pkg_init atomic -∗
@@ -100,74 +131,6 @@ Proof.
   }
 Qed.
 
-Lemma wp_LoadInt32 (addr : loc) dq :
-  ∀ Φ,
-  is_pkg_init atomic -∗
-  (|={⊤,∅}=> ∃ (v : w32), addr ↦{dq} v ∗ (addr ↦{dq} v ={∅,⊤}=∗ Φ #v)) -∗
-  WP @! atomic.LoadInt32 #addr {{ Φ }}.
-Proof.
-  wp_start as "_".
-  iMod "HΦ" as (?) "[Haddr HΦ]".
-  unshelve iApply (wp_typed_Load with "[$]"); try tc_solve; done.
-Qed.
-
-Lemma wp_StoreInt32 (addr : loc) (v : w32) :
-  ∀ Φ,
-  is_pkg_init atomic -∗
-  (|={⊤,∅}=> ∃ (oldv : w32), addr ↦ oldv ∗ (addr ↦ v ={∅,⊤}=∗ Φ #())) -∗
-  WP @! atomic.StoreInt32 #addr #v {{ Φ }}.
-Proof.
-  wp_start as "_".
-  iMod "HΦ" as (?) "[Haddr HΦ]".
-  unshelve iApply (wp_typed_AtomicStore with "[$]"); try tc_solve; done.
-Qed.
-
-Lemma wp_AddInt32 (addr : loc) (v : w32) :
-  ∀ Φ,
-  is_pkg_init atomic -∗
-  (|={⊤,∅}=> ∃ (oldv : w32), addr ↦ oldv ∗ (addr ↦ (word.add oldv v) ={∅,⊤}=∗ Φ #(word.add oldv v))) -∗
-  WP @! atomic.AddInt32 #addr #v {{ Φ }}.
-Proof.
-  wp_start as "_".
-  iMod "HΦ" as (?) "[Haddr HΦ]".
-  rewrite typed_pointsto_unseal /typed_pointsto_def /=.
-  rewrite to_val_unseal /=. rewrite loc_add_0 !right_id.
-  iApply (wp_atomic_op with "Haddr"); first done.
-  iFrame.
-Qed.
-
-Lemma wp_CompareAndSwapInt32 (addr : loc) (old : w32) (new : w32) :
-  ∀ Φ,
-  is_pkg_init atomic -∗
-  (|={⊤,∅}=>
-     ∃ (v: w32) dq,
-     addr ↦{dq} v ∗
-     ⌜ dq = if decide (v = old) then DfracOwn 1 else dq ⌝ ∗
-     (addr ↦{dq} (if decide (v = old) then new else v) ={∅,⊤}=∗ Φ #(bool_decide (v = old)))
-  ) -∗
-  WP @! atomic.CompareAndSwapInt32 #addr #old #new {{ Φ }}.
-Proof.
-  wp_start as "_".
-  wp_bind (CmpXchg _ _ _).
-  iMod "HΦ" as (??) "(? & -> & HΦ)".
-  rewrite bool_decide_decide.
-  destruct decide.
-  {
-    subst.
-    unshelve iApply (wp_typed_cmpxchg_suc with "[$]"); try tc_solve; try done.
-    iIntros "!> ?". iMod ("HΦ" with "[$]"). iModIntro.
-    by wp_auto.
-  }
-  {
-    unshelve iApply (wp_typed_cmpxchg_fail with "[$]"); try tc_solve; try done.
-    { naive_solver. }
-    iIntros "!> ?". iMod ("HΦ" with "[$]"). iModIntro.
-    by wp_auto.
-  }
-Qed.
-
-Definition own_Uint64 (u : loc) dq (v : w64) : iProp Σ :=
-  u ↦{dq} atomic.Uint64.mk (default_val _) (default_val _) v.
 #[global] Opaque own_Uint64.
 #[local] Transparent own_Uint64.
 Global Instance own_Uint64_timeless a b c : Timeless (own_Uint64 a b c) := _.
@@ -209,7 +172,6 @@ Proof.
   wp_auto. done.
 Qed.
 
-
 Lemma wp_Uint64__Store u v :
   ∀ Φ,
   is_pkg_init atomic -∗
@@ -229,7 +191,6 @@ Proof.
 
   iMod ("HΦ" with "[-]").
   {
-    (* FIXME: StructFieldsSplit typeclass is shelved unless something is specified up front. *)
     iApply (struct_fields_combine (V:=atomic.Uint64.t)).
     iFrame.
   }
@@ -258,7 +219,6 @@ Proof.
 
   iMod ("HΦ" with "[-]").
   {
-    (* FIXME: StructFieldsSplit typeclass is shelved unless something is specified up front. *)
     iApply (struct_fields_combine (V:=atomic.Uint64.t)).
     iFrame.
   }
@@ -289,143 +249,593 @@ Proof.
 
   iMod ("HΦ" with "[-]").
   {
-    (* FIXME: StructFieldsSplit typeclass is shelved unless something is specified up front. *)
     iApply (struct_fields_combine (V:=atomic.Uint64.t)).
     iFrame.
   }
   iModIntro.
   wp_auto. done.
 Qed.
+(* END TEMPLATE *)
 
-Definition own_Int32 (u : loc) dq (v : w32) : iProp Σ :=
-  u ↦{dq} atomic.Int32.mk (default_val _) v.
-#[global] Opaque own_Int32.
-#[local] Transparent own_Int32.
-Global Instance own_Int32_timeless a b c : Timeless (own_Int32 a b c) := _.
-Global Instance own_Int32_fractional u v : Fractional (λ q, own_Int32 u (DfracOwn q) v) := _.
-Global Instance own_Int32_as_fractional u q v :
-  AsFractional (own_Int32 u (DfracOwn q) v) (λ q, own_Int32 u (DfracOwn q) v) q := _.
-Global Instance own_Int32_combines_gives u v v' dq dq' :
-  CombineSepGives (own_Int32 u dq v) (own_Int32 u dq' v') (⌜ ✓(dq⋅dq') ∧ v = v'⌝).
-Proof. unfold CombineSepGives.
-  iIntros "?". iDestruct (combine_sep_gives with "[$]") as "#H".
-  rewrite go_type_size_unseal. iDestruct "H" as %?. iModIntro. iPureIntro.
-  naive_solver.
-Qed.
 
-Lemma wp_Int32__Load u dq :
-  ∀ Φ,
-  is_pkg_init atomic -∗
-  (|={⊤,∅}=> ∃ v, own_Int32 u dq v ∗ (own_Int32 u dq v ={∅,⊤}=∗ Φ #v)) -∗
-  WP u @ (ptrT.id atomic.Int32.id) @ "Load" #() {{ Φ }}.
-Proof.
-  wp_start as "_".
-  wp_auto.
-  wp_apply (wp_LoadInt32 with "[$]").
-  iMod "HΦ". iModIntro.
-  iDestruct "HΦ" as (?) "[Hown HΦ]".
-
-  iDestruct (struct_fields_split with "Hown") as "Hl".
-  iNamed "Hl". simpl.
-  iExists _. iFrame.
-  iIntros "Hv".
-
-  iMod ("HΦ" with "[-]").
-  {
-    (* FIXME: StructFieldsSplit typeclass is shelved unless something is specified up front. *)
-    iApply (struct_fields_combine (V:=atomic.Int32.t)).
+(* AUTO-GENERATED - DO NOT EDIT *)
+  (* auto-generated by int_template.py *)
+  (** Int64 *)
+  Lemma wp_LoadInt64 (addr : loc) dq :
+    ∀ Φ,
+    is_pkg_init atomic -∗
+    (|={⊤,∅}=> ∃ (v : w64), addr ↦{dq} v ∗ (addr ↦{dq} v ={∅,⊤}=∗ Φ #v)) -∗
+    WP @! atomic.LoadInt64 #addr {{ Φ }}.
+  Proof.
+    wp_start as "_".
+    iMod "HΦ" as (?) "[Haddr HΦ]".
+    unshelve iApply (wp_typed_Load with "[$]"); try tc_solve; done.
+  Qed.
+  
+  Lemma wp_StoreInt64 (addr : loc) (v : w64) :
+    ∀ Φ,
+    is_pkg_init atomic -∗
+    (|={⊤,∅}=> ∃ (oldv : w64), addr ↦ oldv ∗ (addr ↦ v ={∅,⊤}=∗ Φ #())) -∗
+    WP @! atomic.StoreInt64 #addr #v {{ Φ }}.
+  Proof.
+    wp_start as "_".
+    iMod "HΦ" as (?) "[Haddr HΦ]".
+    unshelve iApply (wp_typed_AtomicStore with "[$]"); try tc_solve; done.
+  Qed.
+  
+  Lemma wp_AddInt64 (addr : loc) (v : w64) :
+    ∀ Φ,
+    is_pkg_init atomic -∗
+    (|={⊤,∅}=> ∃ (oldv : w64), addr ↦ oldv ∗ (addr ↦ (word.add oldv v) ={∅,⊤}=∗ Φ #(word.add oldv v))) -∗
+    WP @! atomic.AddInt64 #addr #v {{ Φ }}.
+  Proof.
+    wp_start as "_".
+    iMod "HΦ" as (?) "[Haddr HΦ]".
+    rewrite typed_pointsto_unseal /typed_pointsto_def /=.
+    rewrite to_val_unseal /=. rewrite loc_add_0 !right_id.
+    iApply (wp_atomic_op with "Haddr"); first done.
     iFrame.
-  }
-  iModIntro.
-  wp_auto. done.
-Qed.
-
-
-Lemma wp_Int32__Store u v :
-  ∀ Φ,
-  is_pkg_init atomic -∗
-  (|={⊤,∅}=> ∃ old, own_Int32 u (DfracOwn 1) old ∗ (own_Int32 u (DfracOwn 1) v ={∅,⊤}=∗ Φ #())) -∗
-  WP u @ (ptrT.id atomic.Int32.id) @ "Store" #v {{ Φ }}.
-Proof.
-  wp_start as "_".
-  wp_auto.
-  wp_apply (wp_StoreInt32 with "[$]").
-  iMod "HΦ". iModIntro.
-  iDestruct "HΦ" as (?) "[Hown HΦ]".
-
-  iDestruct (struct_fields_split with "Hown") as "Hl".
-  iNamed "Hl". simpl.
-  iExists _. iFrame.
-  iIntros "Hv".
-
-  iMod ("HΦ" with "[-]").
-  {
-    (* FIXME: StructFieldsSplit typeclass is shelved unless something is specified up front. *)
-    iApply (struct_fields_combine (V:=atomic.Int32.t)).
+  Qed.
+  
+  Lemma wp_CompareAndSwapInt64 (addr : loc) (old : w64) (new : w64) :
+    ∀ Φ,
+    is_pkg_init atomic -∗
+    (|={⊤,∅}=>
+       ∃ (v: w64) dq,
+       addr ↦{dq} v ∗
+       ⌜ dq = if decide (v = old) then DfracOwn 1 else dq ⌝ ∗
+       (addr ↦{dq} (if decide (v = old) then new else v) ={∅,⊤}=∗ Φ #(bool_decide (v = old)))
+    ) -∗
+    WP @! atomic.CompareAndSwapInt64 #addr #old #new {{ Φ }}.
+  Proof.
+    wp_start as "_".
+    wp_bind (CmpXchg _ _ _).
+    iMod "HΦ" as (??) "(? & -> & HΦ)".
+    rewrite bool_decide_decide.
+    destruct decide.
+    {
+      subst.
+      unshelve iApply (wp_typed_cmpxchg_suc with "[$]"); try tc_solve; try done.
+      iIntros "!> ?". iMod ("HΦ" with "[$]"). iModIntro.
+      by wp_auto.
+    }
+    {
+      unshelve iApply (wp_typed_cmpxchg_fail with "[$]"); try tc_solve; try done.
+      { naive_solver. }
+      iIntros "!> ?". iMod ("HΦ" with "[$]"). iModIntro.
+      by wp_auto.
+    }
+  Qed.
+  
+  #[global] Opaque own_Int64.
+  #[local] Transparent own_Int64.
+  Global Instance own_Int64_timeless a b c : Timeless (own_Int64 a b c) := _.
+  Global Instance own_Int64_fractional u v : Fractional (λ q, own_Int64 u (DfracOwn q) v) := _.
+  Global Instance own_Int64_as_fractional u q v :
+    AsFractional (own_Int64 u (DfracOwn q) v) (λ q, own_Int64 u (DfracOwn q) v) q := _.
+  Global Instance own_Int64_combines_gives u v v' dq dq' :
+    CombineSepGives (own_Int64 u dq v) (own_Int64 u dq' v') (⌜ ✓(dq⋅dq') ∧ v = v'⌝).
+  Proof. unfold CombineSepGives.
+    iIntros "?". iDestruct (combine_sep_gives with "[$]") as "#H".
+    rewrite go_type_size_unseal. iDestruct "H" as %?. iModIntro. iPureIntro.
+    naive_solver.
+  Qed.
+  
+  Lemma wp_Int64__Load u dq :
+    ∀ Φ,
+    is_pkg_init atomic -∗
+    (|={⊤,∅}=> ∃ v, own_Int64 u dq v ∗ (own_Int64 u dq v ={∅,⊤}=∗ Φ #v)) -∗
+    WP u @ (ptrT.id atomic.Int64.id) @ "Load" #() {{ Φ }}.
+  Proof.
+    wp_start as "_".
+    wp_auto.
+    wp_apply (wp_LoadInt64 with "[$]").
+    iMod "HΦ". iModIntro.
+    iDestruct "HΦ" as (?) "[Hown HΦ]".
+  
+    iDestruct (struct_fields_split with "Hown") as "Hl".
+    iNamed "Hl". simpl.
+    iExists _. iFrame.
+    iIntros "Hv".
+  
+    iMod ("HΦ" with "[-]").
+    {
+      (* FIXME: StructFieldsSplit typeclass is shelved unless something is specified up front. *)
+      iApply (struct_fields_combine (V:=atomic.Int64.t)).
+      iFrame.
+    }
+    iModIntro.
+    wp_auto. done.
+  Qed.
+  
+  Lemma wp_Int64__Store u v :
+    ∀ Φ,
+    is_pkg_init atomic -∗
+    (|={⊤,∅}=> ∃ old, own_Int64 u (DfracOwn 1) old ∗ (own_Int64 u (DfracOwn 1) v ={∅,⊤}=∗ Φ #())) -∗
+    WP u @ (ptrT.id atomic.Int64.id) @ "Store" #v {{ Φ }}.
+  Proof.
+    wp_start as "_".
+    wp_auto.
+    wp_apply (wp_StoreInt64 with "[$]").
+    iMod "HΦ". iModIntro.
+    iDestruct "HΦ" as (?) "[Hown HΦ]".
+  
+    iDestruct (struct_fields_split with "Hown") as "Hl".
+    iNamed "Hl". simpl.
+    iExists _. iFrame.
+    iIntros "Hv".
+  
+    iMod ("HΦ" with "[-]").
+    {
+      iApply (struct_fields_combine (V:=atomic.Int64.t)).
+      iFrame.
+    }
+    iModIntro.
+    wp_auto. done.
+  Qed.
+  
+  Lemma wp_Int64__Add u delta :
+    ∀ Φ,
+    is_pkg_init atomic -∗
+    (|={⊤,∅}=> ∃ old, own_Int64 u (DfracOwn 1) old ∗
+    (own_Int64 u (DfracOwn 1) (word.add old delta) ={∅,⊤}=∗
+     Φ #(word.add old delta))) -∗
+    WP u @ (ptrT.id atomic.Int64.id) @ "Add" #delta {{ Φ }}.
+  Proof.
+    wp_start as "_".
+    wp_auto.
+    wp_apply (wp_AddInt64 with "[$]").
+    iMod "HΦ". iModIntro.
+    iDestruct "HΦ" as (?) "[Hown HΦ]".
+  
+    iDestruct (struct_fields_split with "Hown") as "Hl".
+    iNamed "Hl". simpl.
+    iExists _. iFrame.
+    iIntros "Hv".
+  
+    iMod ("HΦ" with "[-]").
+    {
+      iApply (struct_fields_combine (V:=atomic.Int64.t)).
+      iFrame.
+    }
+    iModIntro.
+    wp_auto. done.
+  Qed.
+  
+  Lemma wp_Int64__CompareAndSwap u old new :
+    ∀ Φ,
+    is_pkg_init atomic -∗
+    (|={⊤,∅}=> ∃ v dq, own_Int64 u dq v ∗
+                      ⌜ dq = if decide (v = old) then DfracOwn 1 else dq ⌝ ∗
+    (own_Int64 u dq (if decide (v = old) then new else v) ={∅,⊤}=∗ Φ #(bool_decide (v = old)))) -∗
+    WP u @ (ptrT.id atomic.Int64.id) @ "CompareAndSwap" #old #new {{ Φ }}.
+  Proof.
+    wp_start as "_".
+    wp_auto.
+    wp_apply (wp_CompareAndSwapInt64 with "[$]").
+    iMod "HΦ". iModIntro.
+    iDestruct "HΦ" as (??) "(Hown & -> & HΦ)".
+  
+    iDestruct (struct_fields_split with "Hown") as "Hl".
+    iNamed "Hl". simpl.
+    iExists _. iFrame.
+    iSplitR.
+    { by destruct decide. }
+    iIntros "Hv".
+  
+    iMod ("HΦ" with "[-]").
+    {
+      iApply (struct_fields_combine (V:=atomic.Int64.t)).
+      iFrame.
+    }
+    iModIntro.
+    wp_auto. done.
+  Qed.
+  
+  (** Uint32 *)
+  Lemma wp_LoadUint32 (addr : loc) dq :
+    ∀ Φ,
+    is_pkg_init atomic -∗
+    (|={⊤,∅}=> ∃ (v : w32), addr ↦{dq} v ∗ (addr ↦{dq} v ={∅,⊤}=∗ Φ #v)) -∗
+    WP @! atomic.LoadUint32 #addr {{ Φ }}.
+  Proof.
+    wp_start as "_".
+    iMod "HΦ" as (?) "[Haddr HΦ]".
+    unshelve iApply (wp_typed_Load with "[$]"); try tc_solve; done.
+  Qed.
+  
+  Lemma wp_StoreUint32 (addr : loc) (v : w32) :
+    ∀ Φ,
+    is_pkg_init atomic -∗
+    (|={⊤,∅}=> ∃ (oldv : w32), addr ↦ oldv ∗ (addr ↦ v ={∅,⊤}=∗ Φ #())) -∗
+    WP @! atomic.StoreUint32 #addr #v {{ Φ }}.
+  Proof.
+    wp_start as "_".
+    iMod "HΦ" as (?) "[Haddr HΦ]".
+    unshelve iApply (wp_typed_AtomicStore with "[$]"); try tc_solve; done.
+  Qed.
+  
+  Lemma wp_AddUint32 (addr : loc) (v : w32) :
+    ∀ Φ,
+    is_pkg_init atomic -∗
+    (|={⊤,∅}=> ∃ (oldv : w32), addr ↦ oldv ∗ (addr ↦ (word.add oldv v) ={∅,⊤}=∗ Φ #(word.add oldv v))) -∗
+    WP @! atomic.AddUint32 #addr #v {{ Φ }}.
+  Proof.
+    wp_start as "_".
+    iMod "HΦ" as (?) "[Haddr HΦ]".
+    rewrite typed_pointsto_unseal /typed_pointsto_def /=.
+    rewrite to_val_unseal /=. rewrite loc_add_0 !right_id.
+    iApply (wp_atomic_op with "Haddr"); first done.
     iFrame.
-  }
-  iModIntro.
-  wp_auto. done.
-Qed.
-
-Lemma wp_Int32__Add u delta :
-  ∀ Φ,
-  is_pkg_init atomic -∗
-  (|={⊤,∅}=> ∃ old, own_Int32 u (DfracOwn 1) old ∗
-  (own_Int32 u (DfracOwn 1) (word.add old delta) ={∅,⊤}=∗
-   Φ #(word.add old delta))) -∗
-  WP u @ (ptrT.id atomic.Int32.id) @ "Add" #delta {{ Φ }}.
-Proof.
-  wp_start as "_".
-  wp_auto.
-  wp_apply (wp_AddInt32 with "[$]").
-  iMod "HΦ". iModIntro.
-  iDestruct "HΦ" as (?) "[Hown HΦ]".
-
-  iDestruct (struct_fields_split with "Hown") as "Hl".
-  iNamed "Hl". simpl.
-  iExists _. iFrame.
-  iIntros "Hv".
-
-  iMod ("HΦ" with "[-]").
-  {
-    (* FIXME: StructFieldsSplit typeclass is shelved unless something is specified up front. *)
-    iApply (struct_fields_combine (V:=atomic.Int32.t)).
+  Qed.
+  
+  Lemma wp_CompareAndSwapUint32 (addr : loc) (old : w32) (new : w32) :
+    ∀ Φ,
+    is_pkg_init atomic -∗
+    (|={⊤,∅}=>
+       ∃ (v: w32) dq,
+       addr ↦{dq} v ∗
+       ⌜ dq = if decide (v = old) then DfracOwn 1 else dq ⌝ ∗
+       (addr ↦{dq} (if decide (v = old) then new else v) ={∅,⊤}=∗ Φ #(bool_decide (v = old)))
+    ) -∗
+    WP @! atomic.CompareAndSwapUint32 #addr #old #new {{ Φ }}.
+  Proof.
+    wp_start as "_".
+    wp_bind (CmpXchg _ _ _).
+    iMod "HΦ" as (??) "(? & -> & HΦ)".
+    rewrite bool_decide_decide.
+    destruct decide.
+    {
+      subst.
+      unshelve iApply (wp_typed_cmpxchg_suc with "[$]"); try tc_solve; try done.
+      iIntros "!> ?". iMod ("HΦ" with "[$]"). iModIntro.
+      by wp_auto.
+    }
+    {
+      unshelve iApply (wp_typed_cmpxchg_fail with "[$]"); try tc_solve; try done.
+      { naive_solver. }
+      iIntros "!> ?". iMod ("HΦ" with "[$]"). iModIntro.
+      by wp_auto.
+    }
+  Qed.
+  
+  #[global] Opaque own_Uint32.
+  #[local] Transparent own_Uint32.
+  Global Instance own_Uint32_timeless a b c : Timeless (own_Uint32 a b c) := _.
+  Global Instance own_Uint32_fractional u v : Fractional (λ q, own_Uint32 u (DfracOwn q) v) := _.
+  Global Instance own_Uint32_as_fractional u q v :
+    AsFractional (own_Uint32 u (DfracOwn q) v) (λ q, own_Uint32 u (DfracOwn q) v) q := _.
+  Global Instance own_Uint32_combines_gives u v v' dq dq' :
+    CombineSepGives (own_Uint32 u dq v) (own_Uint32 u dq' v') (⌜ ✓(dq⋅dq') ∧ v = v'⌝).
+  Proof. unfold CombineSepGives.
+    iIntros "?". iDestruct (combine_sep_gives with "[$]") as "#H".
+    rewrite go_type_size_unseal. iDestruct "H" as %?. iModIntro. iPureIntro.
+    naive_solver.
+  Qed.
+  
+  Lemma wp_Uint32__Load u dq :
+    ∀ Φ,
+    is_pkg_init atomic -∗
+    (|={⊤,∅}=> ∃ v, own_Uint32 u dq v ∗ (own_Uint32 u dq v ={∅,⊤}=∗ Φ #v)) -∗
+    WP u @ (ptrT.id atomic.Uint32.id) @ "Load" #() {{ Φ }}.
+  Proof.
+    wp_start as "_".
+    wp_auto.
+    wp_apply (wp_LoadUint32 with "[$]").
+    iMod "HΦ". iModIntro.
+    iDestruct "HΦ" as (?) "[Hown HΦ]".
+  
+    iDestruct (struct_fields_split with "Hown") as "Hl".
+    iNamed "Hl". simpl.
+    iExists _. iFrame.
+    iIntros "Hv".
+  
+    iMod ("HΦ" with "[-]").
+    {
+      (* FIXME: StructFieldsSplit typeclass is shelved unless something is specified up front. *)
+      iApply (struct_fields_combine (V:=atomic.Uint32.t)).
+      iFrame.
+    }
+    iModIntro.
+    wp_auto. done.
+  Qed.
+  
+  Lemma wp_Uint32__Store u v :
+    ∀ Φ,
+    is_pkg_init atomic -∗
+    (|={⊤,∅}=> ∃ old, own_Uint32 u (DfracOwn 1) old ∗ (own_Uint32 u (DfracOwn 1) v ={∅,⊤}=∗ Φ #())) -∗
+    WP u @ (ptrT.id atomic.Uint32.id) @ "Store" #v {{ Φ }}.
+  Proof.
+    wp_start as "_".
+    wp_auto.
+    wp_apply (wp_StoreUint32 with "[$]").
+    iMod "HΦ". iModIntro.
+    iDestruct "HΦ" as (?) "[Hown HΦ]".
+  
+    iDestruct (struct_fields_split with "Hown") as "Hl".
+    iNamed "Hl". simpl.
+    iExists _. iFrame.
+    iIntros "Hv".
+  
+    iMod ("HΦ" with "[-]").
+    {
+      iApply (struct_fields_combine (V:=atomic.Uint32.t)).
+      iFrame.
+    }
+    iModIntro.
+    wp_auto. done.
+  Qed.
+  
+  Lemma wp_Uint32__Add u delta :
+    ∀ Φ,
+    is_pkg_init atomic -∗
+    (|={⊤,∅}=> ∃ old, own_Uint32 u (DfracOwn 1) old ∗
+    (own_Uint32 u (DfracOwn 1) (word.add old delta) ={∅,⊤}=∗
+     Φ #(word.add old delta))) -∗
+    WP u @ (ptrT.id atomic.Uint32.id) @ "Add" #delta {{ Φ }}.
+  Proof.
+    wp_start as "_".
+    wp_auto.
+    wp_apply (wp_AddUint32 with "[$]").
+    iMod "HΦ". iModIntro.
+    iDestruct "HΦ" as (?) "[Hown HΦ]".
+  
+    iDestruct (struct_fields_split with "Hown") as "Hl".
+    iNamed "Hl". simpl.
+    iExists _. iFrame.
+    iIntros "Hv".
+  
+    iMod ("HΦ" with "[-]").
+    {
+      iApply (struct_fields_combine (V:=atomic.Uint32.t)).
+      iFrame.
+    }
+    iModIntro.
+    wp_auto. done.
+  Qed.
+  
+  Lemma wp_Uint32__CompareAndSwap u old new :
+    ∀ Φ,
+    is_pkg_init atomic -∗
+    (|={⊤,∅}=> ∃ v dq, own_Uint32 u dq v ∗
+                      ⌜ dq = if decide (v = old) then DfracOwn 1 else dq ⌝ ∗
+    (own_Uint32 u dq (if decide (v = old) then new else v) ={∅,⊤}=∗ Φ #(bool_decide (v = old)))) -∗
+    WP u @ (ptrT.id atomic.Uint32.id) @ "CompareAndSwap" #old #new {{ Φ }}.
+  Proof.
+    wp_start as "_".
+    wp_auto.
+    wp_apply (wp_CompareAndSwapUint32 with "[$]").
+    iMod "HΦ". iModIntro.
+    iDestruct "HΦ" as (??) "(Hown & -> & HΦ)".
+  
+    iDestruct (struct_fields_split with "Hown") as "Hl".
+    iNamed "Hl". simpl.
+    iExists _. iFrame.
+    iSplitR.
+    { by destruct decide. }
+    iIntros "Hv".
+  
+    iMod ("HΦ" with "[-]").
+    {
+      iApply (struct_fields_combine (V:=atomic.Uint32.t)).
+      iFrame.
+    }
+    iModIntro.
+    wp_auto. done.
+  Qed.
+  
+  (** Int32 *)
+  Lemma wp_LoadInt32 (addr : loc) dq :
+    ∀ Φ,
+    is_pkg_init atomic -∗
+    (|={⊤,∅}=> ∃ (v : w32), addr ↦{dq} v ∗ (addr ↦{dq} v ={∅,⊤}=∗ Φ #v)) -∗
+    WP @! atomic.LoadInt32 #addr {{ Φ }}.
+  Proof.
+    wp_start as "_".
+    iMod "HΦ" as (?) "[Haddr HΦ]".
+    unshelve iApply (wp_typed_Load with "[$]"); try tc_solve; done.
+  Qed.
+  
+  Lemma wp_StoreInt32 (addr : loc) (v : w32) :
+    ∀ Φ,
+    is_pkg_init atomic -∗
+    (|={⊤,∅}=> ∃ (oldv : w32), addr ↦ oldv ∗ (addr ↦ v ={∅,⊤}=∗ Φ #())) -∗
+    WP @! atomic.StoreInt32 #addr #v {{ Φ }}.
+  Proof.
+    wp_start as "_".
+    iMod "HΦ" as (?) "[Haddr HΦ]".
+    unshelve iApply (wp_typed_AtomicStore with "[$]"); try tc_solve; done.
+  Qed.
+  
+  Lemma wp_AddInt32 (addr : loc) (v : w32) :
+    ∀ Φ,
+    is_pkg_init atomic -∗
+    (|={⊤,∅}=> ∃ (oldv : w32), addr ↦ oldv ∗ (addr ↦ (word.add oldv v) ={∅,⊤}=∗ Φ #(word.add oldv v))) -∗
+    WP @! atomic.AddInt32 #addr #v {{ Φ }}.
+  Proof.
+    wp_start as "_".
+    iMod "HΦ" as (?) "[Haddr HΦ]".
+    rewrite typed_pointsto_unseal /typed_pointsto_def /=.
+    rewrite to_val_unseal /=. rewrite loc_add_0 !right_id.
+    iApply (wp_atomic_op with "Haddr"); first done.
     iFrame.
-  }
-  iModIntro.
-  wp_auto. done.
-Qed.
-
-Lemma wp_Int32__CompareAndSwap u old new :
-  ∀ Φ,
-  is_pkg_init atomic -∗
-  (|={⊤,∅}=> ∃ v dq, own_Int32 u dq v ∗
-                    ⌜ dq = if decide (v = old) then DfracOwn 1 else dq ⌝ ∗
-  (own_Int32 u dq (if decide (v = old) then new else v) ={∅,⊤}=∗ Φ #(bool_decide (v = old)))) -∗
-  WP u @ (ptrT.id atomic.Int32.id) @ "CompareAndSwap" #old #new {{ Φ }}.
-Proof.
-  wp_start as "_".
-  wp_auto.
-  wp_apply (wp_CompareAndSwapInt32 with "[$]").
-  iMod "HΦ". iModIntro.
-  iDestruct "HΦ" as (??) "(Hown & -> & HΦ)".
-
-  iDestruct (struct_fields_split with "Hown") as "Hl".
-  iNamed "Hl". simpl.
-  iExists _. iFrame.
-  iSplitR.
-  { by destruct decide. }
-  iIntros "Hv".
-
-  iMod ("HΦ" with "[-]").
-  {
-    (* FIXME: StructFieldsSplit typeclass is shelved unless something is specified up front. *)
-    iApply (struct_fields_combine (V:=atomic.Int32.t)).
-    iFrame.
-  }
-  iModIntro.
-  wp_auto. done.
-Qed.
+  Qed.
+  
+  Lemma wp_CompareAndSwapInt32 (addr : loc) (old : w32) (new : w32) :
+    ∀ Φ,
+    is_pkg_init atomic -∗
+    (|={⊤,∅}=>
+       ∃ (v: w32) dq,
+       addr ↦{dq} v ∗
+       ⌜ dq = if decide (v = old) then DfracOwn 1 else dq ⌝ ∗
+       (addr ↦{dq} (if decide (v = old) then new else v) ={∅,⊤}=∗ Φ #(bool_decide (v = old)))
+    ) -∗
+    WP @! atomic.CompareAndSwapInt32 #addr #old #new {{ Φ }}.
+  Proof.
+    wp_start as "_".
+    wp_bind (CmpXchg _ _ _).
+    iMod "HΦ" as (??) "(? & -> & HΦ)".
+    rewrite bool_decide_decide.
+    destruct decide.
+    {
+      subst.
+      unshelve iApply (wp_typed_cmpxchg_suc with "[$]"); try tc_solve; try done.
+      iIntros "!> ?". iMod ("HΦ" with "[$]"). iModIntro.
+      by wp_auto.
+    }
+    {
+      unshelve iApply (wp_typed_cmpxchg_fail with "[$]"); try tc_solve; try done.
+      { naive_solver. }
+      iIntros "!> ?". iMod ("HΦ" with "[$]"). iModIntro.
+      by wp_auto.
+    }
+  Qed.
+  
+  #[global] Opaque own_Int32.
+  #[local] Transparent own_Int32.
+  Global Instance own_Int32_timeless a b c : Timeless (own_Int32 a b c) := _.
+  Global Instance own_Int32_fractional u v : Fractional (λ q, own_Int32 u (DfracOwn q) v) := _.
+  Global Instance own_Int32_as_fractional u q v :
+    AsFractional (own_Int32 u (DfracOwn q) v) (λ q, own_Int32 u (DfracOwn q) v) q := _.
+  Global Instance own_Int32_combines_gives u v v' dq dq' :
+    CombineSepGives (own_Int32 u dq v) (own_Int32 u dq' v') (⌜ ✓(dq⋅dq') ∧ v = v'⌝).
+  Proof. unfold CombineSepGives.
+    iIntros "?". iDestruct (combine_sep_gives with "[$]") as "#H".
+    rewrite go_type_size_unseal. iDestruct "H" as %?. iModIntro. iPureIntro.
+    naive_solver.
+  Qed.
+  
+  Lemma wp_Int32__Load u dq :
+    ∀ Φ,
+    is_pkg_init atomic -∗
+    (|={⊤,∅}=> ∃ v, own_Int32 u dq v ∗ (own_Int32 u dq v ={∅,⊤}=∗ Φ #v)) -∗
+    WP u @ (ptrT.id atomic.Int32.id) @ "Load" #() {{ Φ }}.
+  Proof.
+    wp_start as "_".
+    wp_auto.
+    wp_apply (wp_LoadInt32 with "[$]").
+    iMod "HΦ". iModIntro.
+    iDestruct "HΦ" as (?) "[Hown HΦ]".
+  
+    iDestruct (struct_fields_split with "Hown") as "Hl".
+    iNamed "Hl". simpl.
+    iExists _. iFrame.
+    iIntros "Hv".
+  
+    iMod ("HΦ" with "[-]").
+    {
+      (* FIXME: StructFieldsSplit typeclass is shelved unless something is specified up front. *)
+      iApply (struct_fields_combine (V:=atomic.Int32.t)).
+      iFrame.
+    }
+    iModIntro.
+    wp_auto. done.
+  Qed.
+  
+  Lemma wp_Int32__Store u v :
+    ∀ Φ,
+    is_pkg_init atomic -∗
+    (|={⊤,∅}=> ∃ old, own_Int32 u (DfracOwn 1) old ∗ (own_Int32 u (DfracOwn 1) v ={∅,⊤}=∗ Φ #())) -∗
+    WP u @ (ptrT.id atomic.Int32.id) @ "Store" #v {{ Φ }}.
+  Proof.
+    wp_start as "_".
+    wp_auto.
+    wp_apply (wp_StoreInt32 with "[$]").
+    iMod "HΦ". iModIntro.
+    iDestruct "HΦ" as (?) "[Hown HΦ]".
+  
+    iDestruct (struct_fields_split with "Hown") as "Hl".
+    iNamed "Hl". simpl.
+    iExists _. iFrame.
+    iIntros "Hv".
+  
+    iMod ("HΦ" with "[-]").
+    {
+      iApply (struct_fields_combine (V:=atomic.Int32.t)).
+      iFrame.
+    }
+    iModIntro.
+    wp_auto. done.
+  Qed.
+  
+  Lemma wp_Int32__Add u delta :
+    ∀ Φ,
+    is_pkg_init atomic -∗
+    (|={⊤,∅}=> ∃ old, own_Int32 u (DfracOwn 1) old ∗
+    (own_Int32 u (DfracOwn 1) (word.add old delta) ={∅,⊤}=∗
+     Φ #(word.add old delta))) -∗
+    WP u @ (ptrT.id atomic.Int32.id) @ "Add" #delta {{ Φ }}.
+  Proof.
+    wp_start as "_".
+    wp_auto.
+    wp_apply (wp_AddInt32 with "[$]").
+    iMod "HΦ". iModIntro.
+    iDestruct "HΦ" as (?) "[Hown HΦ]".
+  
+    iDestruct (struct_fields_split with "Hown") as "Hl".
+    iNamed "Hl". simpl.
+    iExists _. iFrame.
+    iIntros "Hv".
+  
+    iMod ("HΦ" with "[-]").
+    {
+      iApply (struct_fields_combine (V:=atomic.Int32.t)).
+      iFrame.
+    }
+    iModIntro.
+    wp_auto. done.
+  Qed.
+  
+  Lemma wp_Int32__CompareAndSwap u old new :
+    ∀ Φ,
+    is_pkg_init atomic -∗
+    (|={⊤,∅}=> ∃ v dq, own_Int32 u dq v ∗
+                      ⌜ dq = if decide (v = old) then DfracOwn 1 else dq ⌝ ∗
+    (own_Int32 u dq (if decide (v = old) then new else v) ={∅,⊤}=∗ Φ #(bool_decide (v = old)))) -∗
+    WP u @ (ptrT.id atomic.Int32.id) @ "CompareAndSwap" #old #new {{ Φ }}.
+  Proof.
+    wp_start as "_".
+    wp_auto.
+    wp_apply (wp_CompareAndSwapInt32 with "[$]").
+    iMod "HΦ". iModIntro.
+    iDestruct "HΦ" as (??) "(Hown & -> & HΦ)".
+  
+    iDestruct (struct_fields_split with "Hown") as "Hl".
+    iNamed "Hl". simpl.
+    iExists _. iFrame.
+    iSplitR.
+    { by destruct decide. }
+    iIntros "Hv".
+  
+    iMod ("HΦ" with "[-]").
+    {
+      iApply (struct_fields_combine (V:=atomic.Int32.t)).
+      iFrame.
+    }
+    iModIntro.
+    wp_auto. done.
+  Qed.
+  
+(* END AUTO-GENERATED *)
 
 End wps.
